.

Projects/Wuethrich/RunningTime.lean
@@ -3,33 +3,6 @@ import Projects.Wuethrich.Aux
 
 variable {n p : ℕ} [Fact p.Prime] (xs : Vector (ZMod p) (2 ^ n))
 
-def Vector.fntt_auxT {n : ℕ} (xs : Vector (ZMod p) (2 ^ n)) (ω : ZMod p)
-    (powers : Vector (ZMod p) (2 ^ n)) : TimeM (Vector (ZMod p) (2 ^ n)) :=
-  match n with
-  | 0 => pure xs
-  | n + 1 => do
-    let powers' := powers.restrictEven -- Assume this is free
-    let ws := Vector.cast (Nat.min_eq_left (Nat.pow_le_pow_of_le one_lt_two (Nat.le_add_right n 1))) (powers.take (2 ^ n)) -- Assume this is free
-
-    let y_even ← xs.restrictEven.fntt_auxT (ω ^ 2) powers'
-    let y_odd  ← xs.restrictOdd.fntt_auxT (ω ^ 2) powers'
-
-    let left := Vector.zipWith3 (fun e o w ↦ e + w * o) y_even y_odd ws -- Costs O(2 ^ n)
-    let right := Vector.zipWith3 (fun e o w ↦ e - w * o) y_even y_odd ws -- Costs O(2 ^ n)
-
-    let result := (Vector.cast (Eq.symm (Nat.two_pow_succ n)) (left ++ right)) -- Assume this is free
-    ✓ result, (2 ^ (n + 1))
-
-def Vector.fntt_auxT_time (ω : ZMod p) (powers : Vector (ZMod p) (2 ^ n)) :
-    (xs.fntt_auxT ω powers).time = n * 2 ^ n := by
-  induction n generalizing ω with
-  | zero => simp [Vector.fntt_auxT]
-  | succ n ih =>
-    unfold Vector.fntt_auxT
-    simp only [bind, TimeM.tick, take_eq_extract, TimeM.time_of_bind]
-    rw [ih, ih]
-    ring
-
 def getPowersT_loop {p : ℕ} (ω : ZMod p) (size : ℕ) (arr : Array (ZMod p)) (val : ZMod p) : TimeM (Array (ZMod p)) :=
   if arr.size < size then do
       ✓ ()
@@ -38,14 +11,32 @@ def getPowersT_loop {p : ℕ} (ω : ZMod p) (size : ℕ) (arr : Array (ZMod p)) 
     pure arr
 termination_by size - arr.size
 
+theorem getPowersT_loop_time {p : ℕ} (ω : ZMod p) (size : ℕ) (arr : Array (ZMod p)) (val : ZMod p) :
+    (getPowersT_loop ω size arr val).time = size - arr.size := by
+  generalize hg : size - arr.size = gap
+  induction gap generalizing arr val with
+  | zero =>
+    unfold getPowersT_loop
+    rw [Nat.sub_eq_zero_iff_le] at hg
+    simp
+    grind
+  | succ n ih =>
+    unfold getPowersT_loop
+    simp [Nat.lt_of_sub_eq_succ hg]
+    rw [ih]
+    · ring
+    · rw [Array.size_push]
+      omega
+
 def getPowersT (ω : ZMod p) (n : ℕ) : TimeM (Vector (ZMod p) (2 ^ n)) := do
   let initArray := Array.emptyWithCapacity (2 ^ n)
   let arr ← getPowersT_loop ω (2 ^ n) initArray 1
   pure ⟨arr, sorry⟩
 
+theorem getPowersT_time (ω : ZMod p) (n : ℕ) : (getPowersT ω n).time = 2 ^ n := by simp [getPowersT, getPowersT_loop_time]
+
 def Vector.fnttT (ω : ZMod p) : TimeM (Vector (ZMod p) (2 ^ n)) := do
   let powers ← getPowersT ω n
-
   fntt_auxT xs ω powers
   where fntt_auxT {n : ℕ} (xs : Vector (ZMod p) (2 ^ n)) (ω : ZMod p)
     (powers : Vector (ZMod p) (2 ^ n)) : TimeM (Vector (ZMod p) (2 ^ n)) :=
@@ -55,11 +46,26 @@ def Vector.fnttT (ω : ZMod p) : TimeM (Vector (ZMod p) (2 ^ n)) := do
     let powers' := powers.restrictEven -- Assume this is free
     let ws := Vector.cast (Nat.min_eq_left (Nat.pow_le_pow_of_le one_lt_two (Nat.le_add_right n 1))) (powers.take (2 ^ n)) -- Assume this is free
 
-    let y_even ← xs.restrictEven.fntt_auxT (ω ^ 2) powers'
-    let y_odd  ← xs.restrictOdd.fntt_auxT (ω ^ 2) powers'
+    let y_even ← fntt_auxT xs.restrictEven (ω ^ 2) powers'
+    let y_odd  ← fntt_auxT xs.restrictOdd (ω ^ 2) powers'
 
     let left := Vector.zipWith3 (fun e o w ↦ e + w * o) y_even y_odd ws -- Costs O(2 ^ n)
     let right := Vector.zipWith3 (fun e o w ↦ e - w * o) y_even y_odd ws -- Costs O(2 ^ n)
 
     let result := (Vector.cast (Eq.symm (Nat.two_pow_succ n)) (left ++ right)) -- Assume this is free
     ✓ result, (2 ^ (n + 1))
+
+lemma Vector.fntt_auxT_time' (ω : ZMod p) (powers : Vector (ZMod p) (2 ^ n)) :
+    (fnttT.fntt_auxT xs ω powers).time = n * 2 ^ n := by
+  induction n generalizing ω with
+  | zero => simp [fnttT.fntt_auxT]
+  | succ n ih =>
+    unfold fnttT.fntt_auxT
+    simp only [bind, TimeM.tick, take_eq_extract, TimeM.time_of_bind, ih]
+    ring
+
+theorem Vector.fnttT_time (ω : ZMod p)  :
+    (xs.fnttT ω).time = (n + 1) * 2 ^ n := by
+  unfold Vector.fnttT
+  simp [getPowersT_time, Vector.fntt_auxT_time']
+  ring
